veric/mem_lessdef.v
@@ -273,12 +273,473 @@ Proof.
   apply mem_lessalloc_lessdef, mem_equiv_lessalloc, H.
 Qed.
 
+Lemma mem_lessdef_valid_pointer:
+  forall m1 m2 b z, 
+       mem_lessdef m1 m2 ->
+       Mem.valid_pointer m1 b z = true ->
+       Mem.valid_pointer m2 b z = true.
+Proof.
+intros.
+destruct H as [? [? ?]].
+unfold Mem.valid_pointer in *.
+destruct (Mem.perm_dec m1 b z Cur Nonempty); inv H0.
+destruct (Mem.perm_dec m2 b z Cur Nonempty); try reflexivity.
+contradiction n. clear n.
+apply H1; auto.
+Qed.
+
+Lemma mem_lessdef_weak_valid_pointer:
+  forall m1 m2 b z, 
+       mem_lessdef m1 m2 ->
+       Mem.weak_valid_pointer m1 b z = true ->
+       Mem.weak_valid_pointer m2 b z = true.
+Proof.
+intros.
+unfold Mem.weak_valid_pointer in *.
+rewrite orb_true_iff in *.
+destruct H0; [left|right]; eapply mem_lessdef_valid_pointer; eauto.
+Qed.
+
+Lemma mem_lessdef_sem_cast:
+  forall m1 m2, mem_lessdef m1 m2 ->
+  forall v1 v1', Val.lessdef v1 v1' ->
+  forall t1 t2 v, 
+    classify_cast t1 t2 <> cast_case_void ->
+    sem_cast v1 t1 t2 m1 = Some v ->
+    sem_cast v1' t1 t2 m2 = Some v.
+Proof.
+intros until 3. rename H1 into H9. intros.
+unfold sem_cast in *.
+destruct (classify_cast t1 t2) eqn:?HH, v1; inv H1; inv H0; try reflexivity.
+destruct Archi.ptr64 eqn:Hp; inv H3.
+destruct (Mem.weak_valid_pointer m1 b (Ptrofs.unsigned i)) eqn:?; inv H1.
+rewrite (mem_lessdef_weak_valid_pointer _ _ _ _ H Heqb0). auto.
+contradiction H9.
+auto.
+Qed.
+
+Lemma mem_lessdef_sem_binarith:
+  forall m1 m2, mem_lessdef m1 m2 ->
+  forall v1 v1', Val.lessdef v1 v1' ->
+  forall v2 v2', Val.lessdef v2 v2' ->
+  forall (sem_int: signedness -> int -> int -> option val)
+    (sem_long: signedness -> int64 -> int64 -> option val)
+    (sem_float: float -> float -> option val)
+    (sem_single: float32 -> float32 -> option val)
+    (t1: type) (t2: type) v,
+   sem_binarith sem_int sem_long sem_float sem_single v1 t1 v2 t2 m1 = Some v ->
+   sem_binarith sem_int sem_long sem_float sem_single v1' t1 v2' t2 m2 = Some v.
+Proof.
+intros.
+unfold sem_binarith in *.
+destruct (sem_cast v1 t1 (binarith_type (classify_binarith t1 t2)) m1) eqn:?H; try discriminate.
+destruct (sem_cast v2 t2 (binarith_type (classify_binarith t1 t2)) m1) eqn:?H; try discriminate.
+apply (mem_lessdef_sem_cast _ _ H _ _ H0) in H3.
+apply (mem_lessdef_sem_cast _ _ H _ _ H1) in H4.
+rewrite H3, H4.
+auto.
+clear - H2.
+destruct (classify_binarith t1 t2); inv H2; simpl;
+clear; intro;
+destruct t2; try destruct f; try congruence; destruct Archi.ptr64; try congruence.
+destruct (classify_binarith t1 t2); inv H2; simpl;
+clear; intro;
+destruct t1; try destruct f; try congruence; destruct Archi.ptr64; try congruence.
+Qed.
+
+Lemma mem_lessdef_sem_shift:
+  forall m1 m2, mem_lessdef m1 m2 ->
+  forall v1 v1', Val.lessdef v1 v1' ->
+  forall v2 v2', Val.lessdef v2 v2' ->
+  forall (sem_int: signedness -> int -> int -> int)
+    (sem_long: signedness -> int64 -> int64 -> int64)
+    (t1: type) (t2: type) v,
+   sem_shift sem_int sem_long v1 t1 v2 t2 = Some v ->
+   sem_shift sem_int sem_long v1' t1 v2' t2 = Some v.
+Proof.
+intros.
+unfold sem_shift in *.
+destruct (classify_shift t1 t2); auto;
+destruct v1; inv H2; inv H0; destruct v2; inv H4; inv H1; reflexivity.
+Qed.
+
+Lemma mem_lessdef_cmp_ptr:
+  forall m1 m2, mem_lessdef m1 m2 ->
+  forall v1 v1', Val.lessdef v1 v1' ->
+  forall v2 v2', Val.lessdef v2 v2' ->
+  forall op v,
+      cmp_ptr m1 op v1 v2 = Some v ->
+      cmp_ptr m2 op v1' v2' = Some v.
+Proof.
+intros.
+unfold cmp_ptr in *.
+unfold Val.cmpu_bool, Val.cmplu_bool in *.
+destruct Archi.ptr64;
+destruct v1; inv H2; inv H0; destruct v2; inv H4; inv H1; try reflexivity; rewrite H2;
+simpl in *;
+repeat match type of H2 with
+ | context [eq_block ?b ?b0] => destruct (eq_block b b0); [subst b0 |]; simpl in *; try discriminate
+ | context [Int64.eq ?i ?z] => destruct (Int64.eq i z); simpl in *; try discriminate 
+ | context [Mem.valid_pointer m1 ?b ?z] =>
+    let H9 := fresh "H" in 
+    destruct (Mem.valid_pointer m1 b z) eqn:H9; 
+    [ rewrite (mem_lessdef_valid_pointer _ _ _ _ H H9) |  ]
+end;
+rewrite ?andb_false_r in H2;
+try discriminate;
+rewrite ?orb_true_r;
+auto.
+Qed.
+
+Lemma mem_lessdef_sem_cmp:
+  forall m1 m2, mem_lessdef m1 m2 ->
+  forall v1 v1', Val.lessdef v1 v1' ->
+  forall v2 v2', Val.lessdef v2 v2' ->
+  forall op (t1: type) (t2: type) v,
+      sem_cmp op v1 t1 v2 t2 m1 = Some v ->
+      sem_cmp op v1' t1 v2' t2 m2 = Some v.
+Proof.
+intros.
+unfold sem_cmp in *.
+destruct (classify_cmp t1 t2).
+* (* cmp_ptr *)
+eapply mem_lessdef_cmp_ptr; eassumption.
+*
+destruct v2; try discriminate; inv H1.
+eapply mem_lessdef_cmp_ptr; try eassumption; apply Val.lessdef_refl.
+destruct Archi.ptr64; auto.
+eapply mem_lessdef_cmp_ptr; try eassumption; apply Val.lessdef_refl.
+*
+destruct v1; try discriminate; inv H0.
+eapply mem_lessdef_cmp_ptr; try eassumption; apply Val.lessdef_refl.
+destruct Archi.ptr64; auto.
+eapply mem_lessdef_cmp_ptr; try eassumption; apply Val.lessdef_refl.
+*
+destruct v2; try discriminate; inv H1.
+eapply mem_lessdef_cmp_ptr; try eassumption; apply Val.lessdef_refl.
+*
+destruct v1; try discriminate; inv H0.
+eapply mem_lessdef_cmp_ptr; try eassumption; apply Val.lessdef_refl.
+*
+eapply mem_lessdef_sem_binarith; eauto.
+Qed.
+
+Ltac memval_lessdef_tac :=
+match goal with
+ | H: memval_lessdef ?a ?b |- _ => destruct a,b; inv H
+ | H: list_forall2 _ ?a ?b |- _ => destruct a,b; inv H
+ | H: proj_bytes ?a = Some _ |- _ => match a with context [nil] => inv H end
+end;
+ try discriminate;
+ try solve [unfold decode_val; simpl; auto] .
+
+Lemma mem_lessdef_proj_bytes:
+  forall vl vl',
+  list_forall2 memval_lessdef vl vl' ->
+  forall bl, proj_bytes vl = Some bl -> proj_bytes vl' = Some bl.
+Proof.
+intros.
+revert bl H0; induction H; intros; auto.
+destruct bl0; inv H1.
+destruct a1; auto.
+inv H3.
+destruct (proj_bytes al) eqn:?H; inv H3. inv H3.
+destruct a1; try discriminate.
+destruct (proj_bytes al) eqn:?H; inv H3.
+specialize (IHlist_forall2 _ (eq_refl _)).
+inv H.
+simpl.
+rewrite IHlist_forall2.
+auto.
+Qed.
+
+Lemma mem_lessdef_decode_val:
+  forall ch vl vl', list_forall2 memval_lessdef vl vl' ->
+    Val.lessdef (decode_val ch vl) (decode_val ch vl').
+Proof.
+intros.
+unfold decode_val.
+destruct (proj_bytes vl) eqn:?H.
+Focus 2.
+{
+unfold proj_value.
+destruct ch; auto.
++
+destruct Archi.ptr64; auto.
+destruct vl; auto.
+destruct m; auto.
+destruct (check_value (size_quantity_nat Q32) v Q32 (Fragment v q n :: vl)) eqn:?; auto.
+destruct vl'; inv H.
+inv H4.
+unfold proj_bytes.
+destruct (Val.eq v Vundef).
+subst.
+simpl. auto.
+assert (H9: check_value (size_quantity_nat Q32) v2 Q32 (Fragment v2 q n :: vl') = true).
+ 2: rewrite H9; apply Val.load_result_lessdef; apply val_inject_id; auto.
+assert (v2=v).
+apply val_inject_id in H5.
+destruct v; try solve [contradiction n0; auto]; inv H5; auto.
+subst v2.
+clear H5.
+eapply (check_value_inject inject_id); try eassumption.
+constructor; auto.
+constructor; auto.
+apply val_inject_id; apply Val.lessdef_refl.
+apply val_inject_id; apply Val.lessdef_refl.
++
+destruct vl; auto.
+destruct m; auto.
+destruct (check_value (size_quantity_nat Q32) v Q32 (Fragment v q n :: vl)) eqn:?; auto.
+destruct vl'; inv H.
+unfold proj_bytes.
+inv H4.
+destruct (Val.eq v Vundef).
+subst.
+simpl. auto.
+assert (H9: check_value (size_quantity_nat Q32) v2 Q32 (Fragment v2 q n :: vl') = true).
+ 2: rewrite H9; apply Val.load_result_lessdef; apply val_inject_id; auto.
+assert (v2=v).
+apply val_inject_id in H5.
+destruct v; try solve [contradiction n0; auto]; inv H5; auto.
+subst v2.
+clear H5.
+eapply (check_value_inject inject_id); try eassumption.
+constructor; auto.
+constructor; auto.
+apply val_inject_id; apply Val.lessdef_refl.
+apply val_inject_id; apply Val.lessdef_refl.
++
+destruct vl; auto.
+destruct m; auto.
+destruct (check_value (size_quantity_nat Q64) v Q64 (Fragment v q n :: vl)) eqn:?; auto.
+destruct vl'; inv H.
+unfold proj_bytes.
+inv H4.
+destruct (Val.eq v Vundef).
+subst.
+simpl. auto.
+assert (H9: check_value (size_quantity_nat Q64) v2 Q64 (Fragment v2 q n :: vl') = true).
+ 2: rewrite H9; apply Val.load_result_lessdef; apply val_inject_id; auto.
+assert (v2=v).
+apply val_inject_id in H5.
+destruct v; try solve [contradiction n0; auto]; inv H5; auto.
+subst v2.
+clear H5.
+eapply (check_value_inject inject_id); try eassumption.
+constructor; auto.
+constructor; auto.
+apply val_inject_id; apply Val.lessdef_refl.
+apply val_inject_id; apply Val.lessdef_refl.
+} Unfocus.
+rewrite (mem_lessdef_proj_bytes _ _ H _ H0).
+auto.
+Qed.
+
+Lemma classify_cast_void_e:
+ forall t ty, classify_cast t ty = cast_case_void -> ty=Tvoid.
+Proof.
+intros.
+   destruct t as [ | [ | | | ] [ | ] | [ | ] | [ | ] | | | | | ];
+   destruct ty as [ | [ | | | ] [ | ] | [ | ] | [ | ] | | | | | ];
+   inv H; auto.
+Qed.
+
+Lemma mem_lessdef_eval_expr: forall ge ve te m1 m2 a v1,
+   mem_lessdef m1 m2 ->
+   eval_expr ge ve te m1 a v1 -> 
+   exists v2, eval_expr ge ve te m2 a v2 /\ Val.lessdef v1 v2
+ with mem_lessdef_eval_lvalue: forall ge ve te m1 m2 a b z,
+   mem_lessdef m1 m2 ->
+   eval_lvalue ge ve te m1 a b z -> 
+   eval_lvalue ge ve te m2 a b z.
+Proof.
+*
+clear mem_lessdef_eval_expr.
+intros.
+induction H0;
+try solve [eexists; split; [ | eapply Val.lessdef_refl ]; econstructor; eauto].
+destruct IHeval_expr as [vx [? ?]].
+destruct op; simpl in H1.
+ +
+   exists v. split; [ | apply Val.lessdef_refl]. econstructor; simpl; eauto.
+   clear - H1 H3 H.
+   unfold sem_notbool, bool_val in *.
+   destruct (classify_bool (typeof a)), v1; inv H1; inv H3; try reflexivity.
+   destruct Archi.ptr64 eqn:Hp; inv H2.
+   destruct (Mem.weak_valid_pointer m1 b (Ptrofs.unsigned i)) eqn:?; inv H1.
+   rewrite (mem_lessdef_weak_valid_pointer _ _ _ _ H Heqb0). auto.
+ +
+   eexists; split; [ econstructor; eauto; simpl | ].
+  unfold sem_notint in *.
+  destruct (classify_notint (typeof a)); destruct v1; simpl in H1|-*; inv H1; inv H3; reflexivity.
+  apply Val.lessdef_refl.
+ +
+   eexists; split; [ econstructor; eauto; simpl | ].
+  unfold sem_neg in *.
+  destruct (classify_neg (typeof a)); destruct v1; simpl in H1|-*; inv H1; inv H3; reflexivity.
+  apply Val.lessdef_refl.
+ +
+   eexists; split; [ econstructor; eauto; simpl | ].
+  unfold sem_absfloat in *.
+  destruct (classify_neg (typeof a)); destruct v1; simpl in H1|-*; inv H1; inv H3; reflexivity.
+  apply Val.lessdef_refl.
+ +
+   destruct IHeval_expr1 as [?v [? ?]].
+   destruct IHeval_expr2 as [?v [? ?]].
+   rename v0 into v1'. rename v3 into v2'.
+   exists v; split; [ | apply Val.lessdef_refl].
+   econstructor; try eassumption.
+   clear - H0 H2 H4 H.
+   destruct op; simpl in *;
+   try solve [eapply mem_lessdef_sem_binarith; eauto];
+   try solve [eapply mem_lessdef_sem_cmp; eauto].
+   - 
+     unfold sem_add in *. destruct (classify_add (typeof a1) (typeof a2)).
+     destruct v1; inv H0; inv H2; destruct v2; inv H3; inv H4; reflexivity.
+     destruct v1; inv H0; inv H2; destruct v2; inv H3; inv H4; reflexivity.
+     destruct v1; inv H0; inv H2; destruct v2; inv H3; inv H4; reflexivity.
+     destruct v1; inv H0; inv H2; destruct v2; inv H3; inv H4; reflexivity.
+     eapply mem_lessdef_sem_binarith; eauto.
+  - 
+     unfold sem_sub in *. destruct (classify_sub (typeof a1) (typeof a2)).
+     destruct v1; inv H0; inv H2; destruct v2; inv H3; inv H4; reflexivity.
+     destruct v1; inv H0; inv H2; destruct v2; inv H3; inv H4; reflexivity.
+     destruct v1; inv H0; inv H2; destruct v2; inv H3; inv H4; reflexivity.
+     eapply mem_lessdef_sem_binarith; eauto.
+  -
+     eapply mem_lessdef_sem_shift; eauto.
+  -
+     eapply mem_lessdef_sem_shift; eauto.
+ +   
+   destruct IHeval_expr as [v1' [? ?]].
+   destruct (eq_dec ty Tvoid).
+   **
+   subst ty. inv H1.
+   exists v1'. split. subst. econstructor; eauto. auto.
+   **
+   apply (mem_lessdef_sem_cast _ _ H _ _ H3) in H1.
+   exists v. split. econstructor; eauto. apply Val.lessdef_refl.
+   clear - n. contradict n.
+   eapply classify_cast_void_e; eauto.
+ +
+   eapply mem_lessdef_eval_lvalue in H0; eauto.
+   inv H1.
+   2: eexists; split; [eapply eval_Elvalue; eauto; econstructor 2; eassumption | apply Val.lessdef_refl].
+   2: eexists; split; [eapply eval_Elvalue; eauto; econstructor 3; eassumption | apply Val.lessdef_refl].
+   unfold Mem.loadv in *.
+   pose proof (Mem.load_valid_access _ _ _ _ _ H3).
+   destruct H1 as [_ ?].
+   destruct H as [? _].
+   apply Mem.load_loadbytes in H3.
+   destruct H3 as [bytes [? ?]]. apply H in H3.
+   destruct H3 as [v' [? ?]].
+   apply Mem.loadbytes_load in H3; auto.
+   subst.
+   exists (decode_val chunk v').
+   split.
+   eapply eval_Elvalue; eauto.
+   econstructor 1; eauto.
+   clear - H5.
+   apply mem_lessdef_decode_val; auto.
+*
+clear mem_lessdef_eval_lvalue.
+intros.
+induction H0.
+constructor 1; auto.
+constructor 2; auto.
+eapply mem_lessdef_eval_expr in H0; eauto.
+destruct H0 as [v2 [? ?]].
+inv H1.
+econstructor; eauto.
+eapply mem_lessdef_eval_expr in H0; eauto.
+destruct H0 as [v2 [? ?]].
+inv H4.
+econstructor 4; eauto.
+eapply mem_lessdef_eval_expr in H0; eauto.
+destruct H0 as [v2 [? ?]].
+inv H3.
+econstructor 5; eauto.
+Qed.
+
+Lemma mem_lessdef_storebytes:
+  forall m1 m2,   mem_lessdef m1 m2 ->
+  forall v1 v2, list_forall2 memval_lessdef v1 v2 ->
+  forall b z m1', Mem.storebytes m1 b z v1 = Some m1' ->
+  exists m2', mem_lessdef m1' m2' /\ Mem.storebytes m2 b z v2 = Some m2'.
+Admitted.
+
+Lemma mem_lessdef_loadbytes:
+  forall m1 m2, mem_lessdef m1 m2 ->
+  forall b z n v1, Mem.loadbytes m1 b z n = Some v1 ->
+  exists v2, list_forall2 memval_lessdef v1 v2 /\ Mem.loadbytes m2 b z n = Some v2.
+Proof.
+intros.
+destruct H as [? [? ?]].
+apply H in H0.
+destruct H0 as [v2 [? ?]]; exists v2; split; auto.
+Qed.
+
+Lemma mem_lessdef_assign_loc:
+  forall m1 m2,
+  mem_lessdef m1 m2 ->
+  forall ge t loc ofs v m1', 
+  assign_loc ge t m1 loc ofs v m1' ->
+  exists m2', mem_lessdef m1' m2' /\   assign_loc ge t m2 loc ofs v m2'.
+Proof.
+intros.
+inv H0.
+unfold Mem.storev in *.
+exploit Mem.store_valid_access_3. eassumption. intro.
+destruct H0 as [_ ?].
+apply Mem.store_storebytes in H2.
+assert (list_forall2 memval_lessdef (encode_val chunk v) (encode_val chunk v)).
+forget (encode_val chunk v) as bl.
+clear.
+induction bl; simpl. constructor. constructor. apply memval_lessdef_refl. auto.
+destruct (mem_lessdef_storebytes _ _ H _ _ H3 _ _ _ H2) as [m2' [? ?]].
+exists m2'; split; auto. 
+econstructor 1; eauto.
+apply Mem.storebytes_store; auto.
+destruct (mem_lessdef_loadbytes _ _ H _ _ _ _ H5) as [bytes2 [? ?]].
+destruct (mem_lessdef_storebytes _ _ H _ _ H0 _ _ _ H6) as [m2' [? ?]].
+exists m2'; split; auto. 
+econstructor 2; eauto.
+Qed.
+
 Lemma cl_step_mem_lessdef_sim {ge c m1 c' m1' m2} :
   mem_lessdef m1 m2 ->
   @cl_step ge c m1 c' m1' ->
   exists m2',
     mem_lessdef m1' m2' /\
     @cl_step ge c m2 c' m2'.
+Proof.
+intros.
+inv H0.
+* (* step_assign *)
+  eapply mem_lessdef_eval_expr in H3; eauto.
+  eapply mem_lessdef_eval_lvalue in H2; eauto.
+  assert (typeof a1 <> Tvoid).
+  clear - H5; intro. rewrite H in H5. inv H5. inv H0. inv H0.
+  eapply mem_lessdef_sem_cast in H4; eauto.
+  2: contradict H0; eapply classify_cast_void_e; eauto.
+  destruct H3 as [v3 [? ?]].
+  destruct (mem_lessdef_assign_loc _ _ H _ _ _ _ _ _ H5) as [m2' [? ?]].
+  exists m2'.
+  split; auto.
+  econstructor; try eassumption.
+  eapply mem_lessdef_sem_cast in H4; eauto.
+  apply mem_lessalloc_lessdef; apply mem_lessalloc_refl.
+  contradict H0; eapply classify_cast_void_e; eauto.
+* (* step_set *)
+Search mem_lessdef.
+  eapply mem_lessdef_eval_expr in H1; eauto.
+  destruct H1 as [v2 [? ?]].
+  exists m2. split; auto. econstructor.
+  assert (v = v2) by admit. (* not true *)
+  subst v2; auto.
+* (* step_call_internal *)
+  
 Admitted.
 
 Lemma eval_expr_mem_lessaloc {ge ve te m a v}:
